backend/CSEproof.v
@@ -1265,6 +1265,7 @@ Proof.
   econstructor; split.
   eapply exec_Ibuiltin; eauto.
   eapply eval_builtin_args_preserved with (ge1 := ge); eauto. exact allowed_addrof_preserved. exact symbols_preserved.
+  admit.
   eapply external_call_symbols_preserved; eauto. apply senv_preserved.
   rewrite <- comp_transf_function; eauto using allowed_syscall_translated.
   unfold transf_function. unfold analyze in ANALYZE. rewrite ANALYZE; reflexivity.
@@ -1355,6 +1356,7 @@ Proof.
   intros (v' & m1' & P & Q & R & S).
   econstructor; split.
   eapply exec_function_external; eauto.
+  admit.
   eapply external_call_symbols_preserved; eauto. apply senv_preserved.
   (* erewrite <- match_stackframes_call_comp; eauto. *)
   eauto using allowed_syscall_translated.
@@ -1370,7 +1372,7 @@ Proof.
   now eapply return_trace_lessdef; eauto using senv_preserved.
   econstructor; eauto.
   apply set_reg_lessdef; auto.
-Qed.
+Admitted.
 
 Lemma transf_initial_states:
   forall st1, initial_state prog st1 ->
