backend/Deadcodeproof.v
@@ -1264,6 +1264,7 @@ Ltac UseTransfer :=
   eapply eval_builtin_args_preserved with (ge1 := ge) (* (CF1 := @has_comp_fundef _ has_comp_function) *); eauto.
   exact allowed_addrof_preserved.
   exact symbols_preserved.
+  admit.
   rewrite <- comp_transf_function; eauto.
   eapply external_call_symbols_preserved. apply senv_preserved. eauto.
   rewrite <- comp_transf_function; eauto using allowed_syscall_translated.
@@ -1323,6 +1324,7 @@ Ltac UseTransfer :=
   simpl in FUN. inv FUN.
   econstructor; split.
   econstructor; eauto.
+  admit.
   eapply external_call_symbols_preserved; eauto. apply senv_preserved.
   eauto using allowed_syscall_translated.
   econstructor; eauto.
@@ -1336,7 +1338,7 @@ Ltac UseTransfer :=
   rewrite <- comp_transf_function; eauto.
   now eapply return_trace_lessdef; eauto using senv_preserved.
   econstructor; eauto. apply mextends_agree; auto.
-Qed.
+Admitted.
 
 Lemma transf_initial_states:
   forall st1, initial_state prog st1 ->
