backend/Renumberproof.v
@@ -297,6 +297,7 @@ Proof.
   econstructor; split.
   eapply exec_Ibuiltin; eauto.
     eapply eval_builtin_args_preserved with (ge1 := ge); eauto. exact allowed_addrof_preserved. exact symbols_preserved.
+    admit.
     eapply external_call_symbols_preserved; eauto. apply senv_preserved.
     eapply allowed_syscall_translated; eauto.
   constructor; auto. eapply reach_succ; eauto. simpl; auto.
@@ -322,6 +323,7 @@ Proof.
 (* external function *)
   econstructor; split.
   eapply exec_function_external; eauto.
+  admit.
     eapply external_call_symbols_preserved; eauto.
      apply senv_preserved.
      eapply allowed_syscall_translated; eauto.
@@ -333,7 +335,7 @@ Proof.
   rewrite comp_transf_function.
   now eapply return_trace_eq; eauto using senv_preserved.
   constructor; auto.
-Qed.
+Admitted.
 
 Lemma transf_initial_states:
   forall S1, RTL.initial_state prog S1 ->
