backend/SplitLongproof.v
@@ -61,6 +61,7 @@ Ltac DeclHelper := red in HELPERS; decompose [Logic.and] HELPERS; eauto.
 Lemma eval_helper:
   forall bf le id name sg args vargs vres,
   eval_exprlist ge sp e cp m le args vargs ->
+  forall (COND: external_call_conds (EF_runtime name sg) ge cp m vargs),
   helper_declared prog id name sg  ->
   lookup_builtin_function name sg = Some bf ->
   builtin_function_sem bf vargs = Some vres ->
@@ -69,7 +70,7 @@ Proof.
   intros.
   red in H0. apply Genv.find_def_symbol in H0. destruct H0 as (b & P & Q).
   rewrite <- Genv.find_funct_ptr_iff in Q.
-  econstructor; eauto. 
+  econstructor; eauto.
   simpl. red. rewrite H1. constructor; auto.
   unfold Genv.allowed_syscall; auto.
 Qed.
@@ -77,6 +78,7 @@ Qed.
 Corollary eval_helper_1:
   forall bf le id name sg arg1 varg1 vres,
   eval_expr ge sp e cp m le arg1 varg1 ->
+  forall (COND: external_call_conds (EF_runtime name sg) ge cp m (varg1 :: nil)),
   helper_declared prog id name sg  ->
   lookup_builtin_function name sg = Some bf ->
   builtin_function_sem bf (varg1 :: nil) = Some vres ->
@@ -89,6 +91,7 @@ Corollary eval_helper_2:
   forall bf le id name sg arg1 arg2 varg1 varg2 vres,
   eval_expr ge sp e cp m le arg1 varg1 ->
   eval_expr ge sp e cp m le arg2 varg2 ->
+  forall (COND: external_call_conds (EF_runtime name sg) ge cp m (varg1 :: varg2 :: nil)),
   helper_declared prog id name sg  ->
   lookup_builtin_function name sg = Some bf ->
   builtin_function_sem bf (varg1 :: varg2 :: nil) = Some vres ->
@@ -100,12 +103,13 @@ Qed.
 Remark eval_builtin_1:
   forall bf le id sg arg1 varg1 vres,
   eval_expr ge sp e cp m le arg1 varg1 ->
+  forall (COND: external_call_conds (EF_builtin id sg) ge cp m (varg1 :: nil)),
   lookup_builtin_function id sg = Some bf ->
   builtin_function_sem bf (varg1 :: nil) = Some vres ->
   (* forall (ALLOWED: Policy.allowed_call cp (External (EF_builtin id sg))), *)
   eval_expr ge sp e cp m le (Ebuiltin (EF_builtin id sg) (arg1 ::: Enil)) vres.
 Proof.
-  intros. econstructor. econstructor. eauto. constructor.
+  intros. econstructor. econstructor. eauto. constructor. auto.
   simpl. red. rewrite H0. constructor. auto.
   unfold Genv.allowed_syscall; auto.
 Qed.
@@ -114,11 +118,12 @@ Remark eval_builtin_2:
   forall bf le id sg arg1 arg2 varg1 varg2 vres,
   eval_expr ge sp e cp m le arg1 varg1 ->
   eval_expr ge sp e cp m le arg2 varg2 ->
+  forall (COND: external_call_conds (EF_builtin id sg) ge cp m (varg1 :: varg2 :: nil)),
   lookup_builtin_function id sg = Some bf ->
   builtin_function_sem bf (varg1 :: varg2 :: nil) = Some vres ->
   eval_expr ge sp e cp m le (Ebuiltin (EF_builtin id sg) (arg1 ::: arg2 ::: Enil)) vres.
 Proof.
-  intros. econstructor. constructor; eauto. constructor; eauto. constructor.
+  intros. econstructor. constructor; eauto. constructor; eauto. constructor. auto.
   simpl. red. rewrite H1. constructor. auto.
   unfold Genv.allowed_syscall; auto.
 Qed.
@@ -372,7 +377,7 @@ Proof.
 - econstructor; split. apply eval_longconst.
   exploit is_longconst_sound; eauto. intros EQ; subst x. simpl. auto.
 - exists (Val.negl x); split; auto.
-  eapply (eval_builtin_1 (BI_standard BI_negl)); eauto.
+  eapply (eval_builtin_1 (BI_standard BI_negl)); eauto. reflexivity.
 Qed.
 
 Theorem eval_notl: unary_constructor_sound notl Val.notl.
@@ -393,9 +398,8 @@ Theorem eval_longoffloat:
   Val.longoffloat x = Some y ->
   exists v, eval_expr ge sp e cp m le (longoffloat a) v /\ Val.lessdef y v.
 Proof.
-  intros; unfold longoffloat. econstructor; split.
-  eapply (eval_helper_1 (BI_standard BI_i64_dtos)); eauto. DeclHelper. auto.
-  auto.
+  intros; unfold longoffloat. econstructor; split. DeclHelper.
+  eapply (eval_helper_1 (BI_standard BI_i64_dtos)); eauto. reflexivity. auto.
 Qed.
 
 Theorem eval_longuoffloat:
@@ -404,8 +408,8 @@ Theorem eval_longuoffloat:
   Val.longuoffloat x = Some y ->
   exists v, eval_expr ge sp e cp m le (longuoffloat a) v /\ Val.lessdef y v.
 Proof.
-  intros; unfold longuoffloat. econstructor; split.
-  eapply (eval_helper_1 (BI_standard BI_i64_dtou)); eauto. DeclHelper. auto. auto.
+  intros; unfold longuoffloat. econstructor; split. DeclHelper.
+  eapply (eval_helper_1 (BI_standard BI_i64_dtou)); eauto. reflexivity. auto.
 Qed.
 
 Theorem eval_floatoflong:
@@ -414,8 +418,8 @@ Theorem eval_floatoflong:
   Val.floatoflong x = Some y ->
   exists v, eval_expr ge sp e cp m le (floatoflong a) v /\ Val.lessdef y v.
 Proof.
-  intros; unfold floatoflong. exists y; split; auto.
-  eapply (eval_helper_1 (BI_standard BI_i64_stod)); eauto. DeclHelper. auto.
+  intros; unfold floatoflong. exists y; split; auto. DeclHelper.
+  eapply (eval_helper_1 (BI_standard BI_i64_stod)); eauto. reflexivity.
   simpl. destruct x; simpl in H0; inv H0; auto.
 Qed.
 
@@ -425,8 +429,8 @@ Theorem eval_floatoflongu:
   Val.floatoflongu x = Some y ->
   exists v, eval_expr ge sp e cp m le (floatoflongu a) v /\ Val.lessdef y v.
 Proof.
-  intros; unfold floatoflongu. exists y; split; auto.
-  eapply (eval_helper_1 (BI_standard BI_i64_utod)); eauto. DeclHelper. auto.
+  intros; unfold floatoflongu. exists y; split; auto. DeclHelper.
+  eapply (eval_helper_1 (BI_standard BI_i64_utod)); eauto. reflexivity.
   simpl. destruct x; simpl in H0; inv H0; auto.
 Qed.
 
@@ -464,8 +468,8 @@ Theorem eval_singleoflong:
   Val.singleoflong x = Some y ->
   exists v, eval_expr ge sp e cp m le (singleoflong a) v /\ Val.lessdef y v.
 Proof.
-  intros; unfold singleoflong. exists y; split; auto.
-  eapply (eval_helper_1 (BI_standard BI_i64_stof)); eauto. DeclHelper. auto.
+  intros; unfold singleoflong. exists y; split; auto. DeclHelper.
+  eapply (eval_helper_1 (BI_standard BI_i64_stof)); eauto. reflexivity.
   simpl. destruct x; simpl in H0; inv H0; auto.
 Qed.
 
@@ -475,8 +479,8 @@ Theorem eval_singleoflongu:
   Val.singleoflongu x = Some y ->
   exists v, eval_expr ge sp e cp m le (singleoflongu a) v /\ Val.lessdef y v.
 Proof.
-  intros; unfold singleoflongu. exists y; split; auto.
-  eapply (eval_helper_1 (BI_standard BI_i64_utof)); eauto. DeclHelper. auto.
+  intros; unfold singleoflongu. exists y; split; auto. DeclHelper.
+  eapply (eval_helper_1 (BI_standard BI_i64_utof)); eauto. reflexivity.
   simpl. destruct x; simpl in H0; inv H0; auto.
 Qed.
 
@@ -604,8 +608,8 @@ Proof.
     simpl. erewrite <- Int64.decompose_shl_2. instantiate (1 := Int64.hiword i).
     rewrite Int64.ofwords_recompose. auto. auto.
   + (* n >= 64 *)
-    econstructor; split.
-    eapply eval_helper_2; eauto. EvalOp. DeclHelper. reflexivity. reflexivity.
+    econstructor; split. DeclHelper.
+    eapply eval_helper_2; eauto. EvalOp. reflexivity. reflexivity. reflexivity.
     auto.
 Qed.
 
@@ -617,7 +621,7 @@ Proof.
   exploit is_intconst_sound; eauto. intros EQ; subst y; clear H0.
   eapply eval_shllimm; eauto.
 - (* General case *)
-  econstructor; split. eapply eval_helper_2; eauto. DeclHelper. reflexivity. reflexivity. auto.
+  econstructor; split. DeclHelper. eapply eval_helper_2; eauto. reflexivity. reflexivity. reflexivity. auto.
 Qed.
 
 Lemma eval_shrluimm:
@@ -651,8 +655,8 @@ Proof.
     simpl. erewrite <- Int64.decompose_shru_2. instantiate (1 := Int64.loword i).
     rewrite Int64.ofwords_recompose. auto. auto.
   + (* n >= 64 *)
-    econstructor; split.
-    eapply eval_helper_2; eauto. EvalOp. DeclHelper. reflexivity. reflexivity.
+    econstructor; split. DeclHelper.
+    eapply eval_helper_2; eauto. EvalOp. reflexivity. reflexivity. reflexivity.
     auto.
 Qed.
 
@@ -664,7 +668,7 @@ Proof.
   exploit is_intconst_sound; eauto. intros EQ; subst y; clear H0.
   eapply eval_shrluimm; eauto.
 - (* General case *)
-  econstructor; split. eapply eval_helper_2; eauto. DeclHelper. reflexivity. reflexivity. auto.
+  econstructor; split. DeclHelper. eapply eval_helper_2; eauto. reflexivity. reflexivity. reflexivity. auto.
 Qed.
 
 Lemma eval_shrlimm:
@@ -702,8 +706,8 @@ Proof.
     erewrite <- Int64.decompose_shr_2. instantiate (1 := Int64.loword i).
     rewrite Int64.ofwords_recompose. auto. auto.
   + (* n >= 64 *)
-    econstructor; split.
-    eapply eval_helper_2; eauto. EvalOp. DeclHelper. reflexivity. reflexivity.
+    econstructor; split. DeclHelper.
+    eapply eval_helper_2; eauto. EvalOp. reflexivity. reflexivity. reflexivity.
     auto.
 Qed.
 
@@ -715,7 +719,7 @@ Proof.
   exploit is_intconst_sound; eauto. intros EQ; subst y; clear H0.
   eapply eval_shrlimm; eauto.
 - (* General case *)
-  econstructor; split. eapply eval_helper_2; eauto. DeclHelper. reflexivity. reflexivity. auto.
+  econstructor; split. DeclHelper. eapply eval_helper_2; eauto. reflexivity. reflexivity. reflexivity. auto.
 Qed.
 
 Theorem eval_addl: Archi.ptr64 = false -> binary_constructor_sound addl Val.addl.
@@ -725,7 +729,7 @@ Proof.
   assert (DEFAULT:
     exists v, eval_expr ge sp e cp m le default v /\ Val.lessdef (Val.addl x y) v).
   {
-    econstructor; split. eapply eval_builtin_2; eauto. reflexivity. reflexivity. auto.
+    econstructor; split. eapply eval_builtin_2; eauto. reflexivity. reflexivity. reflexivity. auto.
   }
   destruct (is_longconst a) as [p|] eqn:LC1;
   destruct (is_longconst b) as [q|] eqn:LC2.
@@ -748,7 +752,7 @@ Proof.
   assert (DEFAULT:
     exists v, eval_expr ge sp e cp m le default v /\ Val.lessdef (Val.subl x y) v).
   {
-    econstructor; split. eapply eval_builtin_2; eauto. reflexivity. reflexivity. auto.
+    econstructor; split. eapply eval_builtin_2; eauto. reflexivity. reflexivity. reflexivity. auto.
   }
   destruct (is_longconst a) as [p|] eqn:LC1;
   destruct (is_longconst b) as [q|] eqn:LC2.
@@ -779,7 +783,7 @@ Proof.
   exploit eval_add. eexact E2. eexact E3. intros [v5 [E5 L5]].
   exploit eval_add. eexact E5. eexact E4. intros [v6 [E6 L6]].
   exists (Val.longofwords v6 (Val.loword p)); split.
-  EvalOp. eapply eval_builtin_2; eauto. reflexivity. reflexivity. 
+  EvalOp. eapply eval_builtin_2; eauto. reflexivity. reflexivity.  reflexivity.
   intros. unfold le1, p in *; subst; simpl in *.
   inv L3. inv L4. inv L5. simpl in L6. inv L6.
   simpl. f_equal. symmetry. apply Int64.decompose_mul.
@@ -826,15 +830,15 @@ Qed.
 Theorem eval_mullhu:
   forall n, unary_constructor_sound (fun a => mullhu a n) (fun v => Val.mullhu v (Vlong n)).
 Proof.
-  unfold mullhu; intros; red; intros. econstructor; split; eauto.
-  eapply eval_helper_2; eauto. apply eval_longconst. DeclHelper. reflexivity. reflexivity.
+  unfold mullhu; intros; red; intros. econstructor; split; eauto. DeclHelper.
+  eapply eval_helper_2; eauto. apply eval_longconst. reflexivity. reflexivity. reflexivity.
 Qed.
 
 Theorem eval_mullhs:
   forall n, unary_constructor_sound (fun a => mullhs a n) (fun v => Val.mullhs v (Vlong n)).
 Proof.
-  unfold mullhs; intros; red; intros. econstructor; split; eauto.
-  eapply eval_helper_2; eauto. apply eval_longconst. DeclHelper. reflexivity. reflexivity.
+  unfold mullhs; intros; red; intros. econstructor; split; eauto. DeclHelper.
+  eapply eval_helper_2; eauto. apply eval_longconst. reflexivity. reflexivity. reflexivity.
 Qed.
 
 Theorem eval_shrxlimm:
@@ -875,8 +879,8 @@ Theorem eval_divlu_base:
   Val.divlu x y = Some z ->
   exists v, eval_expr ge sp e cp m le (divlu_base a b) v /\ Val.lessdef z v.
 Proof.
-  intros; unfold divlu_base.
-  econstructor; split. eapply eval_helper_2; eauto. DeclHelper. reflexivity. eassumption. auto.
+  intros; unfold divlu_base. DeclHelper.
+  econstructor; split. eapply eval_helper_2; eauto. reflexivity. reflexivity. eassumption. auto.
 Qed.
 
 Theorem eval_modlu_base:
@@ -886,8 +890,8 @@ Theorem eval_modlu_base:
   Val.modlu x y = Some z ->
   exists v, eval_expr ge sp e cp m le (modlu_base a b) v /\ Val.lessdef z v.
 Proof.
-  intros; unfold modlu_base.
-  econstructor; split. eapply eval_helper_2; eauto. DeclHelper. reflexivity. eassumption. auto.
+  intros; unfold modlu_base. DeclHelper.
+  econstructor; split. eapply eval_helper_2; eauto. reflexivity. reflexivity. eassumption. auto.
 Qed.
 
 Theorem eval_divls_base:
@@ -897,8 +901,8 @@ Theorem eval_divls_base:
   Val.divls x y = Some z ->
   exists v, eval_expr ge sp e cp m le (divls_base a b) v /\ Val.lessdef z v.
 Proof.
-  intros; unfold divls_base.
-  econstructor; split. eapply eval_helper_2; eauto. DeclHelper. reflexivity. eassumption. auto.
+  intros; unfold divls_base. DeclHelper.
+  econstructor; split. eapply eval_helper_2; eauto. reflexivity. reflexivity. eassumption. auto.
 Qed.
 
 Theorem eval_modls_base:
@@ -908,8 +912,8 @@ Theorem eval_modls_base:
   Val.modls x y = Some z ->
   exists v, eval_expr ge sp e cp m le (modls_base a b) v /\ Val.lessdef z v.
 Proof.
-  intros; unfold modls_base.
-  econstructor; split. eapply eval_helper_2; eauto. DeclHelper. reflexivity. eassumption. auto.
+  intros; unfold modls_base. DeclHelper.
+  econstructor; split. eapply eval_helper_2; eauto. reflexivity. reflexivity. eassumption. auto.
 Qed.
 
 Remark decompose_cmpl_eq_zero:
