security/BtBasics.v
@@ -48,6 +48,7 @@ Section GENV.
         (p: AST.program F V)
         (NR: list_norepet (prog_defs_names p))
         (AGR: agr_comps p.(prog_pol) (rev (prog_defs p)))
+        (COMPL: pol_complete p.(prog_pol) (rev p.(prog_defs)))
         ge
         (GE: ge = Genv.globalenv p)
         b gd
@@ -56,7 +57,7 @@ Section GENV.
     exists id, Genv.invert_symbol ge b = Some id.
   Proof.
     subst ge. unfold Genv.globalenv, Genv.add_globals, prog_defs_names in *.
-    destruct p; simpl in *. clear - NR AGR DEF.
+    destruct p; simpl in *. clear - AGR COMPL NR DEF.
     remember (Genv.empty_genv F V prog_pol_pub) as ge.
     replace (fold_left (Genv.add_global (V:=V)) prog_defs ge) with
       (fold_right (fun ig g => Genv.add_global g ig) ge (rev prog_defs)) in *.
@@ -65,7 +66,7 @@ Section GENV.
     assert (RNR: list_norepet (map fst rev_prog_defs)).
     { subst. rewrite map_rev. apply list_norepet_rev; auto. }
     clear prog_defs NR Heqrev_prog_defs. subst ge.
-    revert prog_public prog_pol prog_pol_pub b gd DEF AGR RNR.
+    revert prog_public prog_pol prog_pol_pub b gd DEF AGR COMPL RNR.
     induction rev_prog_defs; intros.
     { unfold Genv.find_def in DEF. simpl in DEF. rewrite PTree.gempty in DEF. congruence. }
     destruct a as [id0 gd0].
@@ -73,9 +74,10 @@ Section GENV.
     remember (fold_right (fun (ig : ident * globdef F V) (g : Genv.t F V) => Genv.add_global g ig)
                 (Genv.empty_genv F V prog_pol_pub) rev_prog_defs) as ge.
     assert (AGR': agr_comps prog_pol (rev rev_prog_defs)) by admit.
-    (* assert (GE: ge = Genv.globalenv (AST.mkprogram (rev rev_prog_defs) prog_public id0 prog_pol prog_pol_pub AGR')). *)
-    (* { subst ge. unfold Genv.globalenv. unfold Genv.add_globals. simpl. *)
-    (*   rewrite <- fold_left_rev_right. rewrite rev_involutive. auto. } *)
+    assert (COMPL': pol_complete prog_pol (rev rev_prog_defs)) by admit.
+    assert (GE: ge = Genv.globalenv (AST.mkprogram (rev rev_prog_defs) prog_public id0 prog_pol prog_pol_pub AGR' COMPL')).
+    { subst ge. unfold Genv.globalenv. unfold Genv.add_globals. simpl.
+      rewrite <- fold_left_rev_right. rewrite rev_involutive. auto. }
     apply genv_find_def_add_global_spec in DEF.
     { destruct DEF as [[BLK GD] | [BLK GD]].
       - subst b gd0. exists id0.
@@ -83,22 +85,24 @@ Section GENV.
         rewrite PTree.gss. auto.
       - inversion RNR; clear RNR. subst hd tl.
         assert (AGR'': agr_comps prog_pol rev_prog_defs) by admit.
-        specialize (IHrev_prog_defs _ _ GD AGR'' H2).
+        assert (COMPL'': pol_complete prog_pol rev_prog_defs) by admit.
+        specialize (IHrev_prog_defs _ _ GD AGR'' COMPL'' H2).
         destruct IHrev_prog_defs as [id' INV]. exists id'.
         apply Genv.find_invert_symbol. unfold Genv.find_symbol, Genv.add_global; simpl.
         rewrite PTree.gso. apply Genv.invert_find_symbol in INV. auto.
-        admit.
-        (* clear - H1 Heqge INV . apply Genv.invert_find_symbol in INV. *)
-        (* rewrite GE in INV. apply Genv.find_symbol_inversion in INV. *)
-        (* unfold prog_defs_names in INV. simpl in INV. *)
-        (* rewrite map_rev in INV. apply in_rev in INV. intros CONTRA. subst id'. auto. *)
+        clear - GE H1 Heqge INV. apply Genv.invert_find_symbol in INV.
+        rewrite GE in INV. apply Genv.find_symbol_inversion in INV.
+        unfold prog_defs_names in INV. simpl in INV.
+        rewrite map_rev in INV. apply in_rev in INV. intros CONTRA. subst id'. auto.
     }
-    { destruct (Genv.find_symbol ge id0) eqn:CASE; auto. exfalso.
-      admit.
-      (* rewrite GE in CASE. apply Genv.find_symbol_inversion in CASE. *)
-      (* unfold prog_defs_names in CASE. simpl in CASE. rewrite map_rev in CASE. apply in_rev in CASE. *)
-      (* clear - CASE RNR. inversion RNR. auto. *)
-    }
+    { destruct (Genv.find_symbol ge id0) eqn:CASE; auto.
+      exfalso.
+      rewrite GE in CASE.
+      apply Genv.find_symbol_inversion in CASE.
+      unfold prog_defs_names in CASE.
+      simpl in CASE.
+      rewrite map_rev in CASE. apply in_rev in CASE.
+      clear - CASE RNR. inversion RNR. auto. }
   Admitted.
 
 End GENV.
